libcrux-ml-dsa/proofs/fstar/extraction/Libcrux_ml_dsa.Hash_functions.Portable.fsti
@@ -7,28 +7,89 @@ open FStar.Mul
 type t_Shake128 = | Shake128 : t_Shake128
 
 /// Portable SHAKE 128 x4 state.
-/// We're using a portable implementation so this is actually sequential.
-type t_Shake128X4 = {
-  f_state0:Libcrux_sha3.Portable.t_KeccakState;
-  f_state1:Libcrux_sha3.Portable.t_KeccakState;
-  f_state2:Libcrux_sha3.Portable.t_KeccakState;
-  f_state3:Libcrux_sha3.Portable.t_KeccakState
-}
+/// We\'re using a portable implementation so this is actually sequential.
+val t_Shake128X4:Type0
 
 /// Portable SHAKE 256 state
-type t_Shake256 = { f_state:Libcrux_sha3.Portable.t_KeccakState }
+val t_Shake256:Type0
 
 /// Portable SHAKE 256 x4 state.
-/// We're using a portable implementation so this is actually sequential.
-type t_Shake256X4 = {
-  f_state0:Libcrux_sha3.Portable.t_KeccakState;
-  f_state1:Libcrux_sha3.Portable.t_KeccakState;
-  f_state2:Libcrux_sha3.Portable.t_KeccakState;
-  f_state3:Libcrux_sha3.Portable.t_KeccakState
-}
+/// We\'re using a portable implementation so this is actually sequential.
+val t_Shake256X4:Type0
 
-val init_absorb__init_absorb (input: t_Slice u8)
-    : Prims.Pure Libcrux_sha3.Portable.t_KeccakState Prims.l_True (fun _ -> Prims.l_True)
+val t_Shake256Absorb:Type0
+
+val t_Shake256Squeeze:Type0
+
+val init_absorb (input0 input1 input2 input3: t_Slice u8)
+    : Prims.Pure t_Shake128X4 Prims.l_True (fun _ -> Prims.l_True)
+
+val init_absorb_shake256 (input: t_Slice u8)
+    : Prims.Pure t_Shake256 Prims.l_True (fun _ -> Prims.l_True)
+
+val init_absorb_x4 (input0 input1 input2 input3: t_Slice u8)
+    : Prims.Pure t_Shake256X4 Prims.l_True (fun _ -> Prims.l_True)
+
+val shake128 (v_OUTPUT_LENGTH: usize) (input: t_Slice u8) (out: t_Array u8 v_OUTPUT_LENGTH)
+    : Prims.Pure (t_Array u8 v_OUTPUT_LENGTH) Prims.l_True (fun _ -> Prims.l_True)
+
+[@@ FStar.Tactics.Typeclasses.tcinstance]
+let impl_1: Libcrux_ml_dsa.Hash_functions.Shake128.t_Xof t_Shake128 =
+  {
+    f_shake128_pre
+    =
+    (fun (v_OUTPUT_LENGTH: usize) (input: t_Slice u8) (out: t_Array u8 v_OUTPUT_LENGTH) -> true);
+    f_shake128_post
+    =
+    (fun
+        (v_OUTPUT_LENGTH: usize)
+        (input: t_Slice u8)
+        (out: t_Array u8 v_OUTPUT_LENGTH)
+        (out1: t_Array u8 v_OUTPUT_LENGTH)
+        ->
+        true);
+    f_shake128
+    =
+    fun (v_OUTPUT_LENGTH: usize) (input: t_Slice u8) (out: t_Array u8 v_OUTPUT_LENGTH) ->
+      let out:t_Array u8 v_OUTPUT_LENGTH = shake128 v_OUTPUT_LENGTH input out in
+      out
+  }
+
+val shake256 (v_OUTPUT_LENGTH: usize) (input: t_Slice u8) (out: t_Array u8 v_OUTPUT_LENGTH)
+    : Prims.Pure (t_Array u8 v_OUTPUT_LENGTH) Prims.l_True (fun _ -> Prims.l_True)
+
+val shake256_absorb (st: t_Shake256Absorb) (input: t_Slice u8)
+    : Prims.Pure t_Shake256Absorb Prims.l_True (fun _ -> Prims.l_True)
+
+val shake256_absorb_final (st: t_Shake256Absorb) (input: t_Slice u8)
+    : Prims.Pure t_Shake256Squeeze Prims.l_True (fun _ -> Prims.l_True)
+
+val shake256_init: Prims.unit -> Prims.Pure t_Shake256Absorb Prims.l_True (fun _ -> Prims.l_True)
+
+val shake256_squeeze (st: t_Shake256Squeeze) (out: t_Slice u8)
+    : Prims.Pure (t_Shake256Squeeze & t_Slice u8) Prims.l_True (fun _ -> Prims.l_True)
+
+val squeeze_first_block_shake256 (x: t_Shake256)
+    : Prims.Pure (t_Shake256 & t_Array u8 (sz 136)) Prims.l_True (fun _ -> Prims.l_True)
+
+val squeeze_first_block_x4 (x: t_Shake256X4)
+    : Prims.Pure
+      (t_Shake256X4 &
+        (t_Array u8 (sz 136) & t_Array u8 (sz 136) & t_Array u8 (sz 136) & t_Array u8 (sz 136)))
+      Prims.l_True
+      (fun _ -> Prims.l_True)
+
+val squeeze_first_five_blocks (x: t_Shake128X4) (out0 out1 out2 out3: t_Array u8 (sz 840))
+    : Prims.Pure
+      (t_Shake128X4 & t_Array u8 (sz 840) & t_Array u8 (sz 840) & t_Array u8 (sz 840) &
+        t_Array u8 (sz 840)) Prims.l_True (fun _ -> Prims.l_True)
+
+val squeeze_next_block (x: t_Shake128X4)
+    : Prims.Pure
+      (t_Shake128X4 &
+        (t_Array u8 (sz 168) & t_Array u8 (sz 168) & t_Array u8 (sz 168) & t_Array u8 (sz 168)))
+      Prims.l_True
+      (fun _ -> Prims.l_True)
 
 [@@ FStar.Tactics.Typeclasses.tcinstance]
 let impl: Libcrux_ml_dsa.Hash_functions.Shake128.t_XofX4 t_Shake128X4 =
@@ -50,13 +111,7 @@ let impl: Libcrux_ml_dsa.Hash_functions.Shake128.t_XofX4 t_Shake128X4 =
     f_init_absorb
     =
     (fun (input0: t_Slice u8) (input1: t_Slice u8) (input2: t_Slice u8) (input3: t_Slice u8) ->
-        let state0:Libcrux_sha3.Portable.t_KeccakState = init_absorb__init_absorb input0 in
-        let state1:Libcrux_sha3.Portable.t_KeccakState = init_absorb__init_absorb input1 in
-        let state2:Libcrux_sha3.Portable.t_KeccakState = init_absorb__init_absorb input2 in
-        let state3:Libcrux_sha3.Portable.t_KeccakState = init_absorb__init_absorb input3 in
-        { f_state0 = state0; f_state1 = state1; f_state2 = state2; f_state3 = state3 }
-        <:
-        t_Shake128X4);
+        init_absorb input0 input1 input2 input3);
     f_squeeze_first_five_blocks_pre
     =
     (fun
@@ -89,29 +144,16 @@ let impl: Libcrux_ml_dsa.Hash_functions.Shake128.t_XofX4 t_Shake128X4 =
         (out2: t_Array u8 (sz 840))
         (out3: t_Array u8 (sz 840))
         ->
-        let tmp0, tmp1:(Libcrux_sha3.Portable.t_KeccakState & t_Array u8 (sz 840)) =
-          Libcrux_sha3.Portable.Incremental.shake128_squeeze_first_five_blocks self.f_state0 out0
+        let tmp0, tmp1, tmp2, tmp3, tmp4:(t_Shake128X4 & t_Array u8 (sz 840) & t_Array u8 (sz 840) &
+          t_Array u8 (sz 840) &
+          t_Array u8 (sz 840)) =
+          squeeze_first_five_blocks self out0 out1 out2 out3
         in
-        let self:t_Shake128X4 = { self with f_state0 = tmp0 } <: t_Shake128X4 in
+        let self:t_Shake128X4 = tmp0 in
         let out0:t_Array u8 (sz 840) = tmp1 in
-        let _:Prims.unit = () in
-        let tmp0, tmp1:(Libcrux_sha3.Portable.t_KeccakState & t_Array u8 (sz 840)) =
-          Libcrux_sha3.Portable.Incremental.shake128_squeeze_first_five_blocks self.f_state1 out1
-        in
-        let self:t_Shake128X4 = { self with f_state1 = tmp0 } <: t_Shake128X4 in
-        let out1:t_Array u8 (sz 840) = tmp1 in
-        let _:Prims.unit = () in
-        let tmp0, tmp1:(Libcrux_sha3.Portable.t_KeccakState & t_Array u8 (sz 840)) =
-          Libcrux_sha3.Portable.Incremental.shake128_squeeze_first_five_blocks self.f_state2 out2
-        in
-        let self:t_Shake128X4 = { self with f_state2 = tmp0 } <: t_Shake128X4 in
-        let out2:t_Array u8 (sz 840) = tmp1 in
-        let _:Prims.unit = () in
-        let tmp0, tmp1:(Libcrux_sha3.Portable.t_KeccakState & t_Array u8 (sz 840)) =
-          Libcrux_sha3.Portable.Incremental.shake128_squeeze_first_five_blocks self.f_state3 out3
-        in
-        let self:t_Shake128X4 = { self with f_state3 = tmp0 } <: t_Shake128X4 in
-        let out3:t_Array u8 (sz 840) = tmp1 in
+        let out1:t_Array u8 (sz 840) = tmp2 in
+        let out2:t_Array u8 (sz 840) = tmp3 in
+        let out3:t_Array u8 (sz 840) = tmp4 in
         let _:Prims.unit = () in
         self, out0, out1, out2, out3
         <:
@@ -122,7 +164,7 @@ let impl: Libcrux_ml_dsa.Hash_functions.Shake128.t_XofX4 t_Shake128X4 =
     =
     (fun
         (self: t_Shake128X4)
-        (out4:
+        (out5:
           (t_Shake128X4 &
             (t_Array u8 (sz 168) & t_Array u8 (sz 168) & t_Array u8 (sz 168) & t_Array u8 (sz 168)))
         )
@@ -131,39 +173,14 @@ let impl: Libcrux_ml_dsa.Hash_functions.Shake128.t_XofX4 t_Shake128X4 =
     f_squeeze_next_block
     =
     fun (self: t_Shake128X4) ->
-      let out0:t_Array u8 (sz 168) = Rust_primitives.Hax.repeat 0uy (sz 168) in
-      let tmp0, tmp1:(Libcrux_sha3.Portable.t_KeccakState & t_Array u8 (sz 168)) =
-        Libcrux_sha3.Portable.Incremental.shake128_squeeze_next_block self.f_state0 out0
+      let tmp0, out4:(t_Shake128X4 &
+        (t_Array u8 (sz 168) & t_Array u8 (sz 168) & t_Array u8 (sz 168) & t_Array u8 (sz 168))) =
+        squeeze_next_block self
       in
-      let self:t_Shake128X4 = { self with f_state0 = tmp0 } <: t_Shake128X4 in
-      let out0:t_Array u8 (sz 168) = tmp1 in
-      let _:Prims.unit = () in
-      let out1:t_Array u8 (sz 168) = Rust_primitives.Hax.repeat 0uy (sz 168) in
-      let tmp0, tmp1:(Libcrux_sha3.Portable.t_KeccakState & t_Array u8 (sz 168)) =
-        Libcrux_sha3.Portable.Incremental.shake128_squeeze_next_block self.f_state1 out1
-      in
-      let self:t_Shake128X4 = { self with f_state1 = tmp0 } <: t_Shake128X4 in
-      let out1:t_Array u8 (sz 168) = tmp1 in
-      let _:Prims.unit = () in
-      let out2:t_Array u8 (sz 168) = Rust_primitives.Hax.repeat 0uy (sz 168) in
-      let tmp0, tmp1:(Libcrux_sha3.Portable.t_KeccakState & t_Array u8 (sz 168)) =
-        Libcrux_sha3.Portable.Incremental.shake128_squeeze_next_block self.f_state2 out2
-      in
-      let self:t_Shake128X4 = { self with f_state2 = tmp0 } <: t_Shake128X4 in
-      let out2:t_Array u8 (sz 168) = tmp1 in
-      let _:Prims.unit = () in
-      let out3:t_Array u8 (sz 168) = Rust_primitives.Hax.repeat 0uy (sz 168) in
-      let tmp0, tmp1:(Libcrux_sha3.Portable.t_KeccakState & t_Array u8 (sz 168)) =
-        Libcrux_sha3.Portable.Incremental.shake128_squeeze_next_block self.f_state3 out3
-      in
-      let self:t_Shake128X4 = { self with f_state3 = tmp0 } <: t_Shake128X4 in
-      let out3:t_Array u8 (sz 168) = tmp1 in
-      let _:Prims.unit = () in
+      let self:t_Shake128X4 = tmp0 in
       let hax_temp_output:(t_Array u8 (sz 168) & t_Array u8 (sz 168) & t_Array u8 (sz 168) &
         t_Array u8 (sz 168)) =
-        out0, out1, out2, out3
-        <:
-        (t_Array u8 (sz 168) & t_Array u8 (sz 168) & t_Array u8 (sz 168) & t_Array u8 (sz 168))
+        out4
       in
       self, hax_temp_output
       <:
@@ -171,27 +188,8 @@ let impl: Libcrux_ml_dsa.Hash_functions.Shake128.t_XofX4 t_Shake128X4 =
         (t_Array u8 (sz 168) & t_Array u8 (sz 168) & t_Array u8 (sz 168) & t_Array u8 (sz 168)))
   }
 
-[@@ FStar.Tactics.Typeclasses.tcinstance]
-let impl_1: Libcrux_ml_dsa.Hash_functions.Shake128.t_Xof t_Shake128 =
-  {
-    f_shake128_pre
-    =
-    (fun (v_OUTPUT_LENGTH: usize) (input: t_Slice u8) (out: t_Array u8 v_OUTPUT_LENGTH) -> true);
-    f_shake128_post
-    =
-    (fun
-        (v_OUTPUT_LENGTH: usize)
-        (input: t_Slice u8)
-        (out: t_Array u8 v_OUTPUT_LENGTH)
-        (out1: t_Array u8 v_OUTPUT_LENGTH)
-        ->
-        true);
-    f_shake128
-    =
-    fun (v_OUTPUT_LENGTH: usize) (input: t_Slice u8) (out: t_Array u8 v_OUTPUT_LENGTH) ->
-      let out:t_Array u8 v_OUTPUT_LENGTH = Libcrux_sha3.Portable.shake128 out input in
-      out
-  }
+val squeeze_next_block_shake256 (x: t_Shake256)
+    : Prims.Pure (t_Shake256 & t_Array u8 (sz 136)) Prims.l_True (fun _ -> Prims.l_True)
 
 [@@ FStar.Tactics.Typeclasses.tcinstance]
 let impl_2: Libcrux_ml_dsa.Hash_functions.Shake256.t_Xof t_Shake256 =
@@ -211,53 +209,41 @@ let impl_2: Libcrux_ml_dsa.Hash_functions.Shake256.t_Xof t_Shake256 =
     f_shake256
     =
     (fun (v_OUTPUT_LENGTH: usize) (input: t_Slice u8) (out: t_Array u8 v_OUTPUT_LENGTH) ->
-        let out:t_Array u8 v_OUTPUT_LENGTH = Libcrux_sha3.Portable.shake256 out input in
+        let out:t_Array u8 v_OUTPUT_LENGTH = shake256 v_OUTPUT_LENGTH input out in
         out);
     f_init_absorb_pre = (fun (input: t_Slice u8) -> true);
     f_init_absorb_post = (fun (input: t_Slice u8) (out: t_Shake256) -> true);
-    f_init_absorb
-    =
-    (fun (input: t_Slice u8) ->
-        let state:Libcrux_sha3.Portable.t_KeccakState =
-          Libcrux_sha3.Portable.Incremental.shake256_init ()
-        in
-        let state:Libcrux_sha3.Portable.t_KeccakState =
-          Libcrux_sha3.Portable.Incremental.shake256_absorb_final state input
-        in
-        { f_state = state } <: t_Shake256);
+    f_init_absorb = (fun (input: t_Slice u8) -> init_absorb_shake256 input);
     f_squeeze_first_block_pre = (fun (self: t_Shake256) -> true);
     f_squeeze_first_block_post
     =
-    (fun (self: t_Shake256) (out1: (t_Shake256 & t_Array u8 (sz 136))) -> true);
+    (fun (self: t_Shake256) (out2: (t_Shake256 & t_Array u8 (sz 136))) -> true);
     f_squeeze_first_block
     =
     (fun (self: t_Shake256) ->
-        let out:t_Array u8 (sz 136) = Rust_primitives.Hax.repeat 0uy (sz 136) in
-        let tmp0, tmp1:(Libcrux_sha3.Portable.t_KeccakState & t_Array u8 (sz 136)) =
-          Libcrux_sha3.Portable.Incremental.shake256_squeeze_first_block self.f_state out
-        in
-        let self:t_Shake256 = { self with f_state = tmp0 } <: t_Shake256 in
-        let out:t_Array u8 (sz 136) = tmp1 in
-        let _:Prims.unit = () in
-        let hax_temp_output:t_Array u8 (sz 136) = out in
+        let tmp0, out1:(t_Shake256 & t_Array u8 (sz 136)) = squeeze_first_block_shake256 self in
+        let self:t_Shake256 = tmp0 in
+        let hax_temp_output:t_Array u8 (sz 136) = out1 in
         self, hax_temp_output <: (t_Shake256 & t_Array u8 (sz 136)));
     f_squeeze_next_block_pre = (fun (self: t_Shake256) -> true);
     f_squeeze_next_block_post
     =
-    (fun (self: t_Shake256) (out1: (t_Shake256 & t_Array u8 (sz 136))) -> true);
+    (fun (self: t_Shake256) (out2: (t_Shake256 & t_Array u8 (sz 136))) -> true);
     f_squeeze_next_block
     =
     fun (self: t_Shake256) ->
-      let out:t_Array u8 (sz 136) = Rust_primitives.Hax.repeat 0uy (sz 136) in
-      let tmp0, tmp1:(Libcrux_sha3.Portable.t_KeccakState & t_Array u8 (sz 136)) =
-        Libcrux_sha3.Portable.Incremental.shake256_squeeze_next_block self.f_state out
-      in
-      let self:t_Shake256 = { self with f_state = tmp0 } <: t_Shake256 in
-      let out:t_Array u8 (sz 136) = tmp1 in
-      let _:Prims.unit = () in
-      let hax_temp_output:t_Array u8 (sz 136) = out in
+      let tmp0, out1:(t_Shake256 & t_Array u8 (sz 136)) = squeeze_next_block_shake256 self in
+      let self:t_Shake256 = tmp0 in
+      let hax_temp_output:t_Array u8 (sz 136) = out1 in
       self, hax_temp_output <: (t_Shake256 & t_Array u8 (sz 136))
   }
+
+val squeeze_next_block_x4 (x: t_Shake256X4)
+    : Prims.Pure
+      (t_Shake256X4 &
+        (t_Array u8 (sz 136) & t_Array u8 (sz 136) & t_Array u8 (sz 136) & t_Array u8 (sz 136)))
+      Prims.l_True
+      (fun _ -> Prims.l_True)
 
 [@@ FStar.Tactics.Typeclasses.tcinstance]
 let impl_3: Libcrux_ml_dsa.Hash_functions.Shake256.t_XofX4 t_Shake256X4 =
@@ -279,39 +265,13 @@ let impl_3: Libcrux_ml_dsa.Hash_functions.Shake256.t_XofX4 t_Shake256X4 =
     f_init_absorb_x4
     =
     (fun (input0: t_Slice u8) (input1: t_Slice u8) (input2: t_Slice u8) (input3: t_Slice u8) ->
-        let state0:Libcrux_sha3.Portable.t_KeccakState =
-          Libcrux_sha3.Portable.Incremental.shake256_init ()
-        in
-        let state0:Libcrux_sha3.Portable.t_KeccakState =
-          Libcrux_sha3.Portable.Incremental.shake256_absorb_final state0 input0
-        in
-        let state1:Libcrux_sha3.Portable.t_KeccakState =
-          Libcrux_sha3.Portable.Incremental.shake256_init ()
-        in
-        let state1:Libcrux_sha3.Portable.t_KeccakState =
-          Libcrux_sha3.Portable.Incremental.shake256_absorb_final state1 input1
-        in
-        let state2:Libcrux_sha3.Portable.t_KeccakState =
-          Libcrux_sha3.Portable.Incremental.shake256_init ()
-        in
-        let state2:Libcrux_sha3.Portable.t_KeccakState =
-          Libcrux_sha3.Portable.Incremental.shake256_absorb_final state2 input2
-        in
-        let state3:Libcrux_sha3.Portable.t_KeccakState =
-          Libcrux_sha3.Portable.Incremental.shake256_init ()
-        in
-        let state3:Libcrux_sha3.Portable.t_KeccakState =
-          Libcrux_sha3.Portable.Incremental.shake256_absorb_final state3 input3
-        in
-        { f_state0 = state0; f_state1 = state1; f_state2 = state2; f_state3 = state3 }
-        <:
-        t_Shake256X4);
+        init_absorb_x4 input0 input1 input2 input3);
     f_squeeze_first_block_x4_pre = (fun (self: t_Shake256X4) -> true);
     f_squeeze_first_block_x4_post
     =
     (fun
         (self: t_Shake256X4)
-        (out4:
+        (out5:
           (t_Shake256X4 &
             (t_Array u8 (sz 136) & t_Array u8 (sz 136) & t_Array u8 (sz 136) & t_Array u8 (sz 136)))
         )
@@ -320,39 +280,14 @@ let impl_3: Libcrux_ml_dsa.Hash_functions.Shake256.t_XofX4 t_Shake256X4 =
     f_squeeze_first_block_x4
     =
     (fun (self: t_Shake256X4) ->
-        let out0:t_Array u8 (sz 136) = Rust_primitives.Hax.repeat 0uy (sz 136) in
-        let tmp0, tmp1:(Libcrux_sha3.Portable.t_KeccakState & t_Array u8 (sz 136)) =
-          Libcrux_sha3.Portable.Incremental.shake256_squeeze_first_block self.f_state0 out0
+        let tmp0, out4:(t_Shake256X4 &
+          (t_Array u8 (sz 136) & t_Array u8 (sz 136) & t_Array u8 (sz 136) & t_Array u8 (sz 136))) =
+          squeeze_first_block_x4 self
         in
-        let self:t_Shake256X4 = { self with f_state0 = tmp0 } <: t_Shake256X4 in
-        let out0:t_Array u8 (sz 136) = tmp1 in
-        let _:Prims.unit = () in
-        let out1:t_Array u8 (sz 136) = Rust_primitives.Hax.repeat 0uy (sz 136) in
-        let tmp0, tmp1:(Libcrux_sha3.Portable.t_KeccakState & t_Array u8 (sz 136)) =
-          Libcrux_sha3.Portable.Incremental.shake256_squeeze_first_block self.f_state1 out1
-        in
-        let self:t_Shake256X4 = { self with f_state1 = tmp0 } <: t_Shake256X4 in
-        let out1:t_Array u8 (sz 136) = tmp1 in
-        let _:Prims.unit = () in
-        let out2:t_Array u8 (sz 136) = Rust_primitives.Hax.repeat 0uy (sz 136) in
-        let tmp0, tmp1:(Libcrux_sha3.Portable.t_KeccakState & t_Array u8 (sz 136)) =
-          Libcrux_sha3.Portable.Incremental.shake256_squeeze_first_block self.f_state2 out2
-        in
-        let self:t_Shake256X4 = { self with f_state2 = tmp0 } <: t_Shake256X4 in
-        let out2:t_Array u8 (sz 136) = tmp1 in
-        let _:Prims.unit = () in
-        let out3:t_Array u8 (sz 136) = Rust_primitives.Hax.repeat 0uy (sz 136) in
-        let tmp0, tmp1:(Libcrux_sha3.Portable.t_KeccakState & t_Array u8 (sz 136)) =
-          Libcrux_sha3.Portable.Incremental.shake256_squeeze_first_block self.f_state3 out3
-        in
-        let self:t_Shake256X4 = { self with f_state3 = tmp0 } <: t_Shake256X4 in
-        let out3:t_Array u8 (sz 136) = tmp1 in
-        let _:Prims.unit = () in
+        let self:t_Shake256X4 = tmp0 in
         let hax_temp_output:(t_Array u8 (sz 136) & t_Array u8 (sz 136) & t_Array u8 (sz 136) &
           t_Array u8 (sz 136)) =
-          out0, out1, out2, out3
-          <:
-          (t_Array u8 (sz 136) & t_Array u8 (sz 136) & t_Array u8 (sz 136) & t_Array u8 (sz 136))
+          out4
         in
         self, hax_temp_output
         <:
@@ -363,7 +298,7 @@ let impl_3: Libcrux_ml_dsa.Hash_functions.Shake256.t_XofX4 t_Shake256X4 =
     =
     (fun
         (self: t_Shake256X4)
-        (out4:
+        (out5:
           (t_Shake256X4 &
             (t_Array u8 (sz 136) & t_Array u8 (sz 136) & t_Array u8 (sz 136) & t_Array u8 (sz 136)))
         )
@@ -372,39 +307,14 @@ let impl_3: Libcrux_ml_dsa.Hash_functions.Shake256.t_XofX4 t_Shake256X4 =
     f_squeeze_next_block_x4
     =
     (fun (self: t_Shake256X4) ->
-        let out0:t_Array u8 (sz 136) = Rust_primitives.Hax.repeat 0uy (sz 136) in
-        let tmp0, tmp1:(Libcrux_sha3.Portable.t_KeccakState & t_Array u8 (sz 136)) =
-          Libcrux_sha3.Portable.Incremental.shake256_squeeze_next_block self.f_state0 out0
+        let tmp0, out4:(t_Shake256X4 &
+          (t_Array u8 (sz 136) & t_Array u8 (sz 136) & t_Array u8 (sz 136) & t_Array u8 (sz 136))) =
+          squeeze_next_block_x4 self
         in
-        let self:t_Shake256X4 = { self with f_state0 = tmp0 } <: t_Shake256X4 in
-        let out0:t_Array u8 (sz 136) = tmp1 in
-        let _:Prims.unit = () in
-        let out1:t_Array u8 (sz 136) = Rust_primitives.Hax.repeat 0uy (sz 136) in
-        let tmp0, tmp1:(Libcrux_sha3.Portable.t_KeccakState & t_Array u8 (sz 136)) =
-          Libcrux_sha3.Portable.Incremental.shake256_squeeze_next_block self.f_state1 out1
-        in
-        let self:t_Shake256X4 = { self with f_state1 = tmp0 } <: t_Shake256X4 in
-        let out1:t_Array u8 (sz 136) = tmp1 in
-        let _:Prims.unit = () in
-        let out2:t_Array u8 (sz 136) = Rust_primitives.Hax.repeat 0uy (sz 136) in
-        let tmp0, tmp1:(Libcrux_sha3.Portable.t_KeccakState & t_Array u8 (sz 136)) =
-          Libcrux_sha3.Portable.Incremental.shake256_squeeze_next_block self.f_state2 out2
-        in
-        let self:t_Shake256X4 = { self with f_state2 = tmp0 } <: t_Shake256X4 in
-        let out2:t_Array u8 (sz 136) = tmp1 in
-        let _:Prims.unit = () in
-        let out3:t_Array u8 (sz 136) = Rust_primitives.Hax.repeat 0uy (sz 136) in
-        let tmp0, tmp1:(Libcrux_sha3.Portable.t_KeccakState & t_Array u8 (sz 136)) =
-          Libcrux_sha3.Portable.Incremental.shake256_squeeze_next_block self.f_state3 out3
-        in
-        let self:t_Shake256X4 = { self with f_state3 = tmp0 } <: t_Shake256X4 in
-        let out3:t_Array u8 (sz 136) = tmp1 in
-        let _:Prims.unit = () in
+        let self:t_Shake256X4 = tmp0 in
         let hax_temp_output:(t_Array u8 (sz 136) & t_Array u8 (sz 136) & t_Array u8 (sz 136) &
           t_Array u8 (sz 136)) =
-          out0, out1, out2, out3
-          <:
-          (t_Array u8 (sz 136) & t_Array u8 (sz 136) & t_Array u8 (sz 136) & t_Array u8 (sz 136))
+          out4
         in
         self, hax_temp_output
         <:
@@ -454,10 +364,10 @@ let impl_3: Libcrux_ml_dsa.Hash_functions.Shake256.t_XofX4 t_Shake256X4 =
       (out2: t_Array u8 v_OUT_LEN)
       (out3: t_Array u8 v_OUT_LEN)
       ->
-      let out0:t_Array u8 v_OUT_LEN = Libcrux_sha3.Portable.shake256 out0 input0 in
-      let out1:t_Array u8 v_OUT_LEN = Libcrux_sha3.Portable.shake256 out1 input1 in
-      let out2:t_Array u8 v_OUT_LEN = Libcrux_sha3.Portable.shake256 out2 input2 in
-      let out3:t_Array u8 v_OUT_LEN = Libcrux_sha3.Portable.shake256 out3 input3 in
+      let out0:t_Array u8 v_OUT_LEN = shake256 v_OUT_LEN input0 out0 in
+      let out1:t_Array u8 v_OUT_LEN = shake256 v_OUT_LEN input1 out1 in
+      let out2:t_Array u8 v_OUT_LEN = shake256 v_OUT_LEN input2 out2 in
+      let out3:t_Array u8 v_OUT_LEN = shake256 v_OUT_LEN input3 out3 in
       out0, out1, out2, out3
       <:
       (t_Array u8 v_OUT_LEN & t_Array u8 v_OUT_LEN & t_Array u8 v_OUT_LEN & t_Array u8 v_OUT_LEN)
