libcrux-ml-dsa/proofs/fstar/extraction/Libcrux_ml_dsa.Hash_functions.Simd256.fsti
@@ -6,13 +6,45 @@ open FStar.Mul
 /// AVX2 SHAKE 128 state
 /// This only implements the XofX4 API. For the single Xof, the portable
 /// version is used.
-type t_Shake128x4 = { f_state:Libcrux_sha3.Avx2.X4.Incremental.t_KeccakState }
+val t_Shake128x4:Type0
 
 /// AVX2 SHAKE 256 x4 state.
-type t_Shake256x4 = { f_state:Libcrux_sha3.Avx2.X4.Incremental.t_KeccakState }
+val t_Shake256x4:Type0
 
-/// AVX2 SHAKE 256 state
-type t_Shake256 = { f_state:Libcrux_sha3.Portable.t_KeccakState }
+/// Init the state and absorb 4 blocks in parallel.
+val init_absorb (input0 input1 input2 input3: t_Slice u8)
+    : Prims.Pure t_Shake128x4 Prims.l_True (fun _ -> Prims.l_True)
+
+val init_absorb_x4 (input0 input1 input2 input3: t_Slice u8)
+    : Prims.Pure t_Shake256x4 Prims.l_True (fun _ -> Prims.l_True)
+
+val shake256_x4
+      (v_OUT_LEN: usize)
+      (input0 input1 input2 input3: t_Slice u8)
+      (out0 out1 out2 out3: t_Array u8 v_OUT_LEN)
+    : Prims.Pure
+      (t_Array u8 v_OUT_LEN & t_Array u8 v_OUT_LEN & t_Array u8 v_OUT_LEN & t_Array u8 v_OUT_LEN)
+      Prims.l_True
+      (fun _ -> Prims.l_True)
+
+val squeeze_first_block_x4 (x: t_Shake256x4)
+    : Prims.Pure
+      (t_Shake256x4 &
+        (t_Array u8 (sz 136) & t_Array u8 (sz 136) & t_Array u8 (sz 136) & t_Array u8 (sz 136)))
+      Prims.l_True
+      (fun _ -> Prims.l_True)
+
+val squeeze_first_five_blocks (x: t_Shake128x4) (out0 out1 out2 out3: t_Array u8 (sz 840))
+    : Prims.Pure
+      (t_Shake128x4 & t_Array u8 (sz 840) & t_Array u8 (sz 840) & t_Array u8 (sz 840) &
+        t_Array u8 (sz 840)) Prims.l_True (fun _ -> Prims.l_True)
+
+val squeeze_next_block (x: t_Shake128x4)
+    : Prims.Pure
+      (t_Shake128x4 &
+        (t_Array u8 (sz 168) & t_Array u8 (sz 168) & t_Array u8 (sz 168) & t_Array u8 (sz 168)))
+      Prims.l_True
+      (fun _ -> Prims.l_True)
 
 [@@ FStar.Tactics.Typeclasses.tcinstance]
 let impl: Libcrux_ml_dsa.Hash_functions.Shake128.t_XofX4 t_Shake128x4 =
@@ -34,13 +66,7 @@ let impl: Libcrux_ml_dsa.Hash_functions.Shake128.t_XofX4 t_Shake128x4 =
     f_init_absorb
     =
     (fun (input0: t_Slice u8) (input1: t_Slice u8) (input2: t_Slice u8) (input3: t_Slice u8) ->
-        let state:Libcrux_sha3.Avx2.X4.Incremental.t_KeccakState =
-          Libcrux_sha3.Avx2.X4.Incremental.init ()
-        in
-        let state:Libcrux_sha3.Avx2.X4.Incremental.t_KeccakState =
-          Libcrux_sha3.Avx2.X4.Incremental.shake128_absorb_final state input0 input1 input2 input3
-        in
-        { f_state = state } <: t_Shake128x4);
+        init_absorb input0 input1 input2 input3);
     f_squeeze_first_five_blocks_pre
     =
     (fun
@@ -73,18 +99,12 @@ let impl: Libcrux_ml_dsa.Hash_functions.Shake128.t_XofX4 t_Shake128x4 =
         (out2: t_Array u8 (sz 840))
         (out3: t_Array u8 (sz 840))
         ->
-        let tmp0, tmp1, tmp2, tmp3, tmp4:(Libcrux_sha3.Avx2.X4.Incremental.t_KeccakState &
-          t_Array u8 (sz 840) &
-          t_Array u8 (sz 840) &
+        let tmp0, tmp1, tmp2, tmp3, tmp4:(t_Shake128x4 & t_Array u8 (sz 840) & t_Array u8 (sz 840) &
           t_Array u8 (sz 840) &
           t_Array u8 (sz 840)) =
-          Libcrux_sha3.Avx2.X4.Incremental.shake128_squeeze_first_five_blocks self.f_state
-            out0
-            out1
-            out2
-            out3
+          squeeze_first_five_blocks self out0 out1 out2 out3
         in
-        let self:t_Shake128x4 = { self with f_state = tmp0 } <: t_Shake128x4 in
+        let self:t_Shake128x4 = tmp0 in
         let out0:t_Array u8 (sz 840) = tmp1 in
         let out1:t_Array u8 (sz 840) = tmp2 in
         let out2:t_Array u8 (sz 840) = tmp3 in
@@ -99,7 +119,7 @@ let impl: Libcrux_ml_dsa.Hash_functions.Shake128.t_XofX4 t_Shake128x4 =
     =
     (fun
         (self: t_Shake128x4)
-        (out4:
+        (out5:
           (t_Shake128x4 &
             (t_Array u8 (sz 168) & t_Array u8 (sz 168) & t_Array u8 (sz 168) & t_Array u8 (sz 168)))
         )
@@ -108,32 +128,14 @@ let impl: Libcrux_ml_dsa.Hash_functions.Shake128.t_XofX4 t_Shake128x4 =
     f_squeeze_next_block
     =
     fun (self: t_Shake128x4) ->
-      let out0:t_Array u8 (sz 168) = Rust_primitives.Hax.repeat 0uy (sz 168) in
-      let out1:t_Array u8 (sz 168) = Rust_primitives.Hax.repeat 0uy (sz 168) in
-      let out2:t_Array u8 (sz 168) = Rust_primitives.Hax.repeat 0uy (sz 168) in
-      let out3:t_Array u8 (sz 168) = Rust_primitives.Hax.repeat 0uy (sz 168) in
-      let tmp0, tmp1, tmp2, tmp3, tmp4:(Libcrux_sha3.Avx2.X4.Incremental.t_KeccakState &
-        t_Array u8 (sz 168) &
-        t_Array u8 (sz 168) &
-        t_Array u8 (sz 168) &
-        t_Array u8 (sz 168)) =
-        Libcrux_sha3.Avx2.X4.Incremental.shake128_squeeze_next_block self.f_state
-          out0
-          out1
-          out2
-          out3
+      let tmp0, out4:(t_Shake128x4 &
+        (t_Array u8 (sz 168) & t_Array u8 (sz 168) & t_Array u8 (sz 168) & t_Array u8 (sz 168))) =
+        squeeze_next_block self
       in
-      let self:t_Shake128x4 = { self with f_state = tmp0 } <: t_Shake128x4 in
-      let out0:t_Array u8 (sz 168) = tmp1 in
-      let out1:t_Array u8 (sz 168) = tmp2 in
-      let out2:t_Array u8 (sz 168) = tmp3 in
-      let out3:t_Array u8 (sz 168) = tmp4 in
-      let _:Prims.unit = () in
+      let self:t_Shake128x4 = tmp0 in
       let hax_temp_output:(t_Array u8 (sz 168) & t_Array u8 (sz 168) & t_Array u8 (sz 168) &
         t_Array u8 (sz 168)) =
-        out0, out1, out2, out3
-        <:
-        (t_Array u8 (sz 168) & t_Array u8 (sz 168) & t_Array u8 (sz 168) & t_Array u8 (sz 168))
+        out4
       in
       self, hax_temp_output
       <:
@@ -141,74 +143,15 @@ let impl: Libcrux_ml_dsa.Hash_functions.Shake128.t_XofX4 t_Shake128x4 =
         (t_Array u8 (sz 168) & t_Array u8 (sz 168) & t_Array u8 (sz 168) & t_Array u8 (sz 168)))
   }
 
-[@@ FStar.Tactics.Typeclasses.tcinstance]
-let impl_1: Libcrux_ml_dsa.Hash_functions.Shake256.t_Xof t_Shake256 =
-  {
-    f_shake256_pre
-    =
-    (fun (v_OUTPUT_LENGTH: usize) (input: t_Slice u8) (out: t_Array u8 v_OUTPUT_LENGTH) -> true);
-    f_shake256_post
-    =
-    (fun
-        (v_OUTPUT_LENGTH: usize)
-        (input: t_Slice u8)
-        (out: t_Array u8 v_OUTPUT_LENGTH)
-        (out1: t_Array u8 v_OUTPUT_LENGTH)
-        ->
-        true);
-    f_shake256
-    =
-    (fun (v_OUTPUT_LENGTH: usize) (input: t_Slice u8) (out: t_Array u8 v_OUTPUT_LENGTH) ->
-        let out:t_Array u8 v_OUTPUT_LENGTH = Libcrux_sha3.Portable.shake256 out input in
-        out);
-    f_init_absorb_pre = (fun (input: t_Slice u8) -> true);
-    f_init_absorb_post = (fun (input: t_Slice u8) (out: t_Shake256) -> true);
-    f_init_absorb
-    =
-    (fun (input: t_Slice u8) ->
-        let state:Libcrux_sha3.Portable.t_KeccakState =
-          Libcrux_sha3.Portable.Incremental.shake256_init ()
-        in
-        let state:Libcrux_sha3.Portable.t_KeccakState =
-          Libcrux_sha3.Portable.Incremental.shake256_absorb_final state input
-        in
-        { f_state = state } <: t_Shake256);
-    f_squeeze_first_block_pre = (fun (self: t_Shake256) -> true);
-    f_squeeze_first_block_post
-    =
-    (fun (self: t_Shake256) (out1: (t_Shake256 & t_Array u8 (sz 136))) -> true);
-    f_squeeze_first_block
-    =
-    (fun (self: t_Shake256) ->
-        let out:t_Array u8 (sz 136) = Rust_primitives.Hax.repeat 0uy (sz 136) in
-        let tmp0, tmp1:(Libcrux_sha3.Portable.t_KeccakState & t_Array u8 (sz 136)) =
-          Libcrux_sha3.Portable.Incremental.shake256_squeeze_first_block self.f_state out
-        in
-        let self:t_Shake256 = { self with f_state = tmp0 } <: t_Shake256 in
-        let out:t_Array u8 (sz 136) = tmp1 in
-        let _:Prims.unit = () in
-        let hax_temp_output:t_Array u8 (sz 136) = out in
-        self, hax_temp_output <: (t_Shake256 & t_Array u8 (sz 136)));
-    f_squeeze_next_block_pre = (fun (self: t_Shake256) -> true);
-    f_squeeze_next_block_post
-    =
-    (fun (self: t_Shake256) (out1: (t_Shake256 & t_Array u8 (sz 136))) -> true);
-    f_squeeze_next_block
-    =
-    fun (self: t_Shake256) ->
-      let out:t_Array u8 (sz 136) = Rust_primitives.Hax.repeat 0uy (sz 136) in
-      let tmp0, tmp1:(Libcrux_sha3.Portable.t_KeccakState & t_Array u8 (sz 136)) =
-        Libcrux_sha3.Portable.Incremental.shake256_squeeze_next_block self.f_state out
-      in
-      let self:t_Shake256 = { self with f_state = tmp0 } <: t_Shake256 in
-      let out:t_Array u8 (sz 136) = tmp1 in
-      let _:Prims.unit = () in
-      let hax_temp_output:t_Array u8 (sz 136) = out in
-      self, hax_temp_output <: (t_Shake256 & t_Array u8 (sz 136))
-  }
+val squeeze_next_block_x4 (x: t_Shake256x4)
+    : Prims.Pure
+      (t_Shake256x4 &
+        (t_Array u8 (sz 136) & t_Array u8 (sz 136) & t_Array u8 (sz 136) & t_Array u8 (sz 136)))
+      Prims.l_True
+      (fun _ -> Prims.l_True)
 
 [@@ FStar.Tactics.Typeclasses.tcinstance]
-let impl_2: Libcrux_ml_dsa.Hash_functions.Shake256.t_XofX4 t_Shake256x4 =
+let impl_1: Libcrux_ml_dsa.Hash_functions.Shake256.t_XofX4 t_Shake256x4 =
   {
     f_init_absorb_x4_pre
     =
@@ -227,19 +170,13 @@ let impl_2: Libcrux_ml_dsa.Hash_functions.Shake256.t_XofX4 t_Shake256x4 =
     f_init_absorb_x4
     =
     (fun (input0: t_Slice u8) (input1: t_Slice u8) (input2: t_Slice u8) (input3: t_Slice u8) ->
-        let state:Libcrux_sha3.Avx2.X4.Incremental.t_KeccakState =
-          Libcrux_sha3.Avx2.X4.Incremental.init ()
-        in
-        let state:Libcrux_sha3.Avx2.X4.Incremental.t_KeccakState =
-          Libcrux_sha3.Avx2.X4.Incremental.shake256_absorb_final state input0 input1 input2 input3
-        in
-        { f_state = state } <: t_Shake256x4);
+        init_absorb_x4 input0 input2 input2 input3);
     f_squeeze_first_block_x4_pre = (fun (self: t_Shake256x4) -> true);
     f_squeeze_first_block_x4_post
     =
     (fun
         (self: t_Shake256x4)
-        (out4:
+        (out5:
           (t_Shake256x4 &
             (t_Array u8 (sz 136) & t_Array u8 (sz 136) & t_Array u8 (sz 136) & t_Array u8 (sz 136)))
         )
@@ -248,32 +185,14 @@ let impl_2: Libcrux_ml_dsa.Hash_functions.Shake256.t_XofX4 t_Shake256x4 =
     f_squeeze_first_block_x4
     =
     (fun (self: t_Shake256x4) ->
-        let out0:t_Array u8 (sz 136) = Rust_primitives.Hax.repeat 0uy (sz 136) in
-        let out1:t_Array u8 (sz 136) = Rust_primitives.Hax.repeat 0uy (sz 136) in
-        let out2:t_Array u8 (sz 136) = Rust_primitives.Hax.repeat 0uy (sz 136) in
-        let out3:t_Array u8 (sz 136) = Rust_primitives.Hax.repeat 0uy (sz 136) in
-        let tmp0, tmp1, tmp2, tmp3, tmp4:(Libcrux_sha3.Avx2.X4.Incremental.t_KeccakState &
-          t_Array u8 (sz 136) &
-          t_Array u8 (sz 136) &
-          t_Array u8 (sz 136) &
-          t_Array u8 (sz 136)) =
-          Libcrux_sha3.Avx2.X4.Incremental.shake256_squeeze_first_block self.f_state
-            out0
-            out1
-            out2
-            out3
+        let tmp0, out4:(t_Shake256x4 &
+          (t_Array u8 (sz 136) & t_Array u8 (sz 136) & t_Array u8 (sz 136) & t_Array u8 (sz 136))) =
+          squeeze_first_block_x4 self
         in
-        let self:t_Shake256x4 = { self with f_state = tmp0 } <: t_Shake256x4 in
-        let out0:t_Array u8 (sz 136) = tmp1 in
-        let out1:t_Array u8 (sz 136) = tmp2 in
-        let out2:t_Array u8 (sz 136) = tmp3 in
-        let out3:t_Array u8 (sz 136) = tmp4 in
-        let _:Prims.unit = () in
+        let self:t_Shake256x4 = tmp0 in
         let hax_temp_output:(t_Array u8 (sz 136) & t_Array u8 (sz 136) & t_Array u8 (sz 136) &
           t_Array u8 (sz 136)) =
-          out0, out1, out2, out3
-          <:
-          (t_Array u8 (sz 136) & t_Array u8 (sz 136) & t_Array u8 (sz 136) & t_Array u8 (sz 136))
+          out4
         in
         self, hax_temp_output
         <:
@@ -284,7 +203,7 @@ let impl_2: Libcrux_ml_dsa.Hash_functions.Shake256.t_XofX4 t_Shake256x4 =
     =
     (fun
         (self: t_Shake256x4)
-        (out4:
+        (out5:
           (t_Shake256x4 &
             (t_Array u8 (sz 136) & t_Array u8 (sz 136) & t_Array u8 (sz 136) & t_Array u8 (sz 136)))
         )
@@ -293,32 +212,14 @@ let impl_2: Libcrux_ml_dsa.Hash_functions.Shake256.t_XofX4 t_Shake256x4 =
     f_squeeze_next_block_x4
     =
     (fun (self: t_Shake256x4) ->
-        let out0:t_Array u8 (sz 136) = Rust_primitives.Hax.repeat 0uy (sz 136) in
-        let out1:t_Array u8 (sz 136) = Rust_primitives.Hax.repeat 0uy (sz 136) in
-        let out2:t_Array u8 (sz 136) = Rust_primitives.Hax.repeat 0uy (sz 136) in
-        let out3:t_Array u8 (sz 136) = Rust_primitives.Hax.repeat 0uy (sz 136) in
-        let tmp0, tmp1, tmp2, tmp3, tmp4:(Libcrux_sha3.Avx2.X4.Incremental.t_KeccakState &
-          t_Array u8 (sz 136) &
-          t_Array u8 (sz 136) &
-          t_Array u8 (sz 136) &
-          t_Array u8 (sz 136)) =
-          Libcrux_sha3.Avx2.X4.Incremental.shake256_squeeze_next_block self.f_state
-            out0
-            out1
-            out2
-            out3
+        let tmp0, out4:(t_Shake256x4 &
+          (t_Array u8 (sz 136) & t_Array u8 (sz 136) & t_Array u8 (sz 136) & t_Array u8 (sz 136))) =
+          squeeze_next_block_x4 self
         in
-        let self:t_Shake256x4 = { self with f_state = tmp0 } <: t_Shake256x4 in
-        let out0:t_Array u8 (sz 136) = tmp1 in
-        let out1:t_Array u8 (sz 136) = tmp2 in
-        let out2:t_Array u8 (sz 136) = tmp3 in
-        let out3:t_Array u8 (sz 136) = tmp4 in
-        let _:Prims.unit = () in
+        let self:t_Shake256x4 = tmp0 in
         let hax_temp_output:(t_Array u8 (sz 136) & t_Array u8 (sz 136) & t_Array u8 (sz 136) &
           t_Array u8 (sz 136)) =
-          out0, out1, out2, out3
-          <:
-          (t_Array u8 (sz 136) & t_Array u8 (sz 136) & t_Array u8 (sz 136) & t_Array u8 (sz 136))
+          out4
         in
         self, hax_temp_output
         <:
@@ -370,7 +271,7 @@ let impl_2: Libcrux_ml_dsa.Hash_functions.Shake256.t_XofX4 t_Shake256x4 =
       ->
       let tmp0, tmp1, tmp2, tmp3:(t_Array u8 v_OUT_LEN & t_Array u8 v_OUT_LEN & t_Array u8 v_OUT_LEN &
         t_Array u8 v_OUT_LEN) =
-        Libcrux_sha3.Avx2.X4.shake256 input0 input1 input2 input3 out0 out1 out2 out3
+        shake256_x4 v_OUT_LEN input0 input1 input2 input3 out0 out1 out2 out3
       in
       let out0:t_Array u8 v_OUT_LEN = tmp0 in
       let out1:t_Array u8 v_OUT_LEN = tmp1 in
