libcrux-ml-dsa/proofs/fstar/extraction/Libcrux_ml_dsa.Ml_dsa_generic.Instantiations.Avx2.fst
@@ -6,6 +6,7 @@ open FStar.Mul
 let _ =
   (* This module has implicit dependencies, here we make them explicit. *)
   (* The implicit dependencies arise from typeclasses instances. *)
+  let open Libcrux_ml_dsa.Hash_functions.Portable in
   let open Libcrux_ml_dsa.Hash_functions.Shake128 in
   let open Libcrux_ml_dsa.Hash_functions.Shake256 in
   let open Libcrux_ml_dsa.Hash_functions.Simd256 in
@@ -21,7 +22,7 @@ let generate_key_pair
      =
   Libcrux_ml_dsa.Ml_dsa_generic.generate_key_pair #Libcrux_ml_dsa.Simd.Avx2.Vector_type.t_AVX2SIMDUnit
     #Libcrux_ml_dsa.Hash_functions.Simd256.t_Shake128x4
-    #Libcrux_ml_dsa.Hash_functions.Simd256.t_Shake256
+    #Libcrux_ml_dsa.Hash_functions.Portable.t_Shake256
     #Libcrux_ml_dsa.Hash_functions.Simd256.t_Shake256x4 v_ROWS_IN_A v_COLUMNS_IN_A v_ETA
     v_ERROR_RING_ELEMENT_SIZE v_SIGNING_KEY_SIZE v_VERIFICATION_KEY_SIZE randomness
 
@@ -36,7 +37,7 @@ let sign
      =
   Libcrux_ml_dsa.Ml_dsa_generic.sign #Libcrux_ml_dsa.Simd.Avx2.Vector_type.t_AVX2SIMDUnit
     #Libcrux_ml_dsa.Hash_functions.Simd256.t_Shake128x4
-    #Libcrux_ml_dsa.Hash_functions.Simd256.t_Shake256
+    #Libcrux_ml_dsa.Hash_functions.Portable.t_Shake256
     #Libcrux_ml_dsa.Hash_functions.Simd256.t_Shake256x4 v_ROWS_IN_A v_COLUMNS_IN_A v_ETA
     v_ERROR_RING_ELEMENT_SIZE v_GAMMA1_EXPONENT v_GAMMA2 v_COMMITMENT_RING_ELEMENT_SIZE
     v_COMMITMENT_VECTOR_SIZE v_COMMITMENT_HASH_SIZE v_ONES_IN_VERIFIER_CHALLENGE v_MAX_ONES_IN_HINT
@@ -54,7 +55,7 @@ let sign_pre_hashed_shake128
      =
   Libcrux_ml_dsa.Ml_dsa_generic.sign_pre_hashed #Libcrux_ml_dsa.Simd.Avx2.Vector_type.t_AVX2SIMDUnit
     #Libcrux_ml_dsa.Hash_functions.Simd256.t_Shake128x4
-    #Libcrux_ml_dsa.Hash_functions.Simd256.t_Shake256
+    #Libcrux_ml_dsa.Hash_functions.Portable.t_Shake256
     #Libcrux_ml_dsa.Hash_functions.Simd256.t_Shake256x4 #Libcrux_ml_dsa.Pre_hash.t_SHAKE128_PH
     (sz 256) v_ROWS_IN_A v_COLUMNS_IN_A v_ETA v_ERROR_RING_ELEMENT_SIZE v_GAMMA1_EXPONENT v_GAMMA2
     v_COMMITMENT_RING_ELEMENT_SIZE v_COMMITMENT_VECTOR_SIZE v_COMMITMENT_HASH_SIZE
@@ -73,7 +74,7 @@ let verify
      =
   Libcrux_ml_dsa.Ml_dsa_generic.verify #Libcrux_ml_dsa.Simd.Avx2.Vector_type.t_AVX2SIMDUnit
     #Libcrux_ml_dsa.Hash_functions.Simd256.t_Shake128x4
-    #Libcrux_ml_dsa.Hash_functions.Simd256.t_Shake256 v_ROWS_IN_A v_COLUMNS_IN_A v_SIGNATURE_SIZE
+    #Libcrux_ml_dsa.Hash_functions.Portable.t_Shake256 v_ROWS_IN_A v_COLUMNS_IN_A v_SIGNATURE_SIZE
     v_VERIFICATION_KEY_SIZE v_GAMMA1_EXPONENT v_GAMMA1_RING_ELEMENT_SIZE v_GAMMA2 v_BETA
     v_COMMITMENT_RING_ELEMENT_SIZE v_COMMITMENT_VECTOR_SIZE v_COMMITMENT_HASH_SIZE
     v_ONES_IN_VERIFIER_CHALLENGE v_MAX_ONES_IN_HINT verification_key message context signature
@@ -90,7 +91,7 @@ let verify_pre_hashed_shake128
      =
   Libcrux_ml_dsa.Ml_dsa_generic.verify_pre_hashed #Libcrux_ml_dsa.Simd.Avx2.Vector_type.t_AVX2SIMDUnit
     #Libcrux_ml_dsa.Hash_functions.Simd256.t_Shake128x4
-    #Libcrux_ml_dsa.Hash_functions.Simd256.t_Shake256 #Libcrux_ml_dsa.Pre_hash.t_SHAKE128_PH
+    #Libcrux_ml_dsa.Hash_functions.Portable.t_Shake256 #Libcrux_ml_dsa.Pre_hash.t_SHAKE128_PH
     (sz 256) v_ROWS_IN_A v_COLUMNS_IN_A v_SIGNATURE_SIZE v_VERIFICATION_KEY_SIZE v_GAMMA1_EXPONENT
     v_GAMMA1_RING_ELEMENT_SIZE v_GAMMA2 v_BETA v_COMMITMENT_RING_ELEMENT_SIZE
     v_COMMITMENT_VECTOR_SIZE v_COMMITMENT_HASH_SIZE v_ONES_IN_VERIFIER_CHALLENGE v_MAX_ONES_IN_HINT
